filled in a lemma about refinement

src/temporal_logic/pair.lean
@@ -7,7 +7,7 @@ open predicate
 
 section pair
 
-variables {α' : Type u} {β' : Type u₀} {γ' : Type u₁}
+variables {α' : Type u} {β' : Type u₀} {γ' : Type u₁} {ω : Type u₂}
 variables (x : tvar α') (y : tvar β') (z : tvar γ')
 
 @[simp]
@@ -19,6 +19,10 @@ by { cases x, cases y, refl }
 def pair.fst : var (α' × β') α' :=
 ⟨ @prod.fst α' β' ⟩
 
+@[reducible]
+def pair.snd : var (α' × β') β' :=
+⟨ @prod.snd α' β' ⟩
+
 @[simp]
 def pair.fst_mk (x : tvar α') (y : tvar β')
 : pair.fst ! ⦃y,x⦄ = x :=
@@ -28,6 +32,11 @@ by lifted_pred
 def pair.fst_mk' (x : tvar α') (y : tvar β')
 : ⟨ @prod.fst α' β' ⟩ ! ⦃y,x⦄ = x :=
 pair.fst_mk _ _
+
+@[simp]
+def pair.snd_mk (x : tvar α') (y : tvar β')
+: pair.snd ! ⦃y,x⦄ = y :=
+by lifted_pred
 
 @[simp]
 def pair.snd_mk' (x : tvar α') (y : tvar β')
@@ -52,6 +61,16 @@ by ext i ; simp [map_right]
 lemma map_left_proj_pair (f : α' → γ')
 : ⟨map_left f⟩ ! ⦃y,x⦄ = ⦃y, ⟨f⟩ ! x⦄ :=
 by ext i ; simp [map_left]
+
+@[simp]
+lemma map_proj_pair (f : α' → γ') (g : β' → ω)
+: ⟨prod.map f g⟩ ! ⦃y,x⦄ = ⦃⟨g⟩ ! y, ⟨f⟩ ! x⦄ :=
+by ext i ; simp [prod.map]
+
+@[simp]
+lemma eta_pair (w : tvar (α' × β'))
+: ⦃pair.snd ! w, pair.fst ! w⦄ = w :=
+by ext i ; simp [prod.map]
 
 @[simp]
 lemma next_pair (v₀ : tvar α') (v₁ : tvar β')
